ViewsProof.v
@@ -52,115 +52,40 @@ Proposition preserveInjectivity_is_correct :
   forall A B (f : ViewArray A -> ViewArray B), preserveInjectivity f -> (forall v, Injective v -> Injective (f v)).
 Proof.
   unfold preserveInjectivity.
-  intros.
+  intros A B f Hf v Hinj x y.
   unfold Injective.
   intros.
-  apply H with (C := Nil nat) (x := x) (y := y) (i := I) (j := I) in H0.
-  destruct H0.
-  apply H2.
-  simpl. apply H1.
+  apply Hf with (C := Nil nat) (x := x) (y := y) (i := I) (j := I) in H.
+  destruct H as [_ H].
+  apply H.
+  simpl. apply Hinj.
 Qed.
 
 Proposition to_view_injective :
   forall n, Injective (to_view n).
 Proof.
   unfold Injective.
-  intros.
+  intros n x y H.
   unfold to_view in H.
   simpl in H.
-  destruct x,y.
+  destruct x as [x tx],y as [y ty].
   apply to_nat_injective in H.
-  destruct t,t0.
+  destruct tx,ty.
   rewrite H.
   reflexivity.
 Qed.
 
-Proposition reverse_preserves_injectivity :
-  forall T n (v : ViewArray[[T;n]]), Injective v -> Injective (reverse v).
-Proof.
-  unfold Injective.
-  intros.
-  unfold reverse in *.
-  destruct x as [x tx],y as [y ty].
-  simpl in *.
-  apply H with (x := ((Id n (n - 1 - to_nat x) reverseProof),tx)) (y := ((Id n (n - 1 - to_nat y) reverseProof),ty)) in H0.
-  injection H0.
-  intros.
-  apply sub_injective in H2.
-  apply to_nat_injective in H2. subst. reflexivity.
-  destruct n. destruct x. inversion H3. simpl. rewrite Nat.sub_0_r. apply le_S_n. apply BoundedInt.
-  destruct n. destruct y. inversion H3. simpl. rewrite Nat.sub_0_r. apply le_S_n. apply BoundedInt.
-Qed.
-
-Proposition select_preserves_injectivity :
-  forall T n (a : nat) (b : nat) (v : ViewArray[[T;b+n]]), Injective v -> Injective (select a b v).
-Proof.
-  unfold Injective.
-  intros.
-  unfold select in H0.
-  simpl in H0.
-  destruct x as [x tx],y as [y ty].
-  apply H with (x := ((Id (b + n) (a + to_nat x) selectProof),tx)) (y := ((Id (b + n) (a + to_nat y) selectProof),ty)) in H0.
-  injection H0. intros.
-  apply add_injective in H2.
-  apply to_nat_injective in H2.
-  subst. reflexivity.
-Qed.
-
-Proposition transpose_preserves_injectivity :
-  forall T n m (v : ViewArray[[[[T;n]];m]]), Injective v -> Injective (transpose v).
-Proof.
-  unfold Injective.
-  intros.
-  unfold transpose in *.
-  destruct x as [ix tx], y as [iy ty], tx as [jx tx], ty as [jy ty].
-  simpl in *.
-  apply H with (x := (jx,(ix,tx))) (y := (jy,(iy,ty))) in H0.
-  injection H0.
-  intros.
-  subst. reflexivity.
-Qed.
-
-Proposition group_preserves_injectivity :
-  forall T n m (v : ViewArray[[T;m*n]]), Injective v -> Injective (group m v).
-Proof.
-  unfold Injective.
-  intros.
-  unfold group in *.
-  destruct x as [ix tx], y as [iy ty], tx as [jx tx], ty as [jy ty].
-  simpl in *.
-  apply H with (x := ((Id (m * n) (to_nat jx + m * to_nat ix) groupProof),tx)) (y := ((Id (m * n) (to_nat jy + m * to_nat iy) groupProof),ty)) in H0.
-  inversion H0.
-  apply projection_injective in H2.
-  inversion H2.
-  apply to_nat_injective in H4, H5.
-  subst. reflexivity.
-  apply BoundedInt.
-  apply BoundedInt.
-Qed.
-
 Lemma reorder_is_correct :
   forall C A (n : nat) (v : ViewArray (C++(n::A))) (i : Tuple C) (x : Idx n),
-  curry_partialApp v i x = curry_partialApp (reorder v) (A := (n::C)) (x,i).
+  curry_partialApp v i x = curry_partialApp (reorder v x) i.
 Proof.
   intros.
   induction C.
   - simpl. reflexivity.
-  - destruct i. simpl.
+  - destruct i as [i t]. simpl.
   assert ((curry_partialApp (v i) t x) = curry_partialApp (reorder (v i)) (A := n::C) (B := A) (x, t)).
   apply IHC.
   rewrite H. simpl. reflexivity.
-Qed.
-
-Lemma reorder_is_correct_2 :
-  forall C A (n : nat) (v : ViewArray (C++(n::A))) (i : Tuple C) (x : Idx n),
-  curry_partialApp (reorder v x) i = curry_partialApp v i x.
-Proof.
-  intros.
-  induction C.
-  - simpl. reflexivity.
-  - destruct i. simpl.
-  apply IHC.
 Qed.
 
 Lemma decomposition :
@@ -171,17 +96,17 @@ Proof.
   intros.
   induction C.
   - simpl in *. exists I,x. split; reflexivity.
-  - simpl. destruct x.
-  assert (exists (i0 : Tuple C) (j : Tuple A),
-        curry_totalApp (v i) t = curry_totalApp (curry_partialApp (v i) i0) j /\ t = tupcat i0 j).
+  - simpl. destruct x as [x tx].
+  assert (exists (i : Tuple C) (j : Tuple A),
+        curry_totalApp (v x) tx = curry_totalApp (curry_partialApp (v x) i) j /\ tx = tupcat i j).
   apply IHC.
-  destruct H.
-  destruct H.
-  exists (i,x).
-  exists x0.
+  destruct H as [c H].
+  destruct H as [a H].
+  exists (x,c).
+  exists a.
   split.
   apply H.
-  assert (t = tupcat x x0). apply H.
+  assert (tx = tupcat c a). apply H.
   subst. reflexivity.
 Qed.
 
@@ -204,7 +129,7 @@ Proof.
   - destruct x1,x2. simpl in H. subst. reflexivity.
   - destruct x1 as [x1 tx1],x2 as [x2 tx2].
   simpl in H.
-  injection H. intros. apply IHA in H0. inversion H0. subst. reflexivity.
+  injection H. intros Htupcat Hx. apply IHA in Htupcat. inversion Htupcat. subst. reflexivity.
 Qed.
 
 Proposition reorder_keeps_injectivity :
@@ -213,12 +138,12 @@ Proposition reorder_keeps_injectivity :
 Proof.
   intros C A.
   destruct C.
-  - intros. simpl in *. unfold Injective in *.
-    intros. simpl in *.
-    apply H in H0.
-    apply H0.
+  - intros n v Hinj. simpl in *. unfold Injective in *.
+    intros x y H. simpl in *.
+    apply Hinj in H.
+    apply H.
   - unfold Injective.
-    intros.
+    intros n v Hinj x y H.
     destruct x as [x1 tx],y as [y1 ty].
     destruct tx as [x2 tx], ty as [y2 ty].
     assert (Hx:exists (i : Tuple (n::h::C)) (j : Tuple A),
@@ -230,8 +155,8 @@ Proof.
     destruct ix as [ix1 tix].
     destruct tix as [ix2 tix].
     destruct Hx as [Hx Hi].
-    rewrite reorder_is_correct_2 in Hx.
-    rewrite Hx in H0.
+    rewrite <- reorder_is_correct in Hx.
+    rewrite Hx in H.
     assert (Hy:exists (i : Tuple (n::h::C)) (j : Tuple A),
     curry_totalApp (reorder v (C:=h::C)) (y1, (y2, ty)) = curry_totalApp (curry_partialApp (reorder v (C := h::C)) (A := n::h::C) i) j
     /\ (y1,(y2,ty)) = tupcat i j).
@@ -241,22 +166,22 @@ Proof.
     destruct iy as [iy1 tiy].
     destruct tiy as [iy2 tiy].
     destruct Hy as [Hy Hj].
-    rewrite reorder_is_correct_2 in Hy.
-    rewrite Hy in H0.
-    assert (curry_totalApp (curry_partialApp v (A := (h::C)) (ix2,tix)) (ix1,jx) = curry_totalApp v (A := ((h::C)++(n::A))) (tupcat (ix2,tix) (A:=(h::C)) (ix1,jx) (B:=(n::A)))).
+    rewrite <- reorder_is_correct in Hy.
+    rewrite Hy in H.
+    clear Hx. clear Hy.
+    assert (Hx:curry_totalApp (curry_partialApp v (A := (h::C)) (ix2,tix)) (ix1,jx) = curry_totalApp v (A := ((h::C)++(n::A))) (tupcat (ix2,tix) (A:=(h::C)) (ix1,jx) (B:=(n::A)))).
     symmetry. apply recomposition with (i := (ix2,tix)) (j := (ix1,jx)).
-    simpl in H1. rewrite H1 in H0.
-    assert (curry_totalApp (curry_partialApp v (A := (h::C)) (iy2,tiy)) (iy1,jy) = curry_totalApp v (A := ((h::C)++(n::A))) (tupcat (iy2,tiy) (A:=(h::C)) (iy1,jy) (B:=(n::A)))).
+    simpl in Hx. rewrite Hx in H.
+    assert (Hy:curry_totalApp (curry_partialApp v (A := (h::C)) (iy2,tiy)) (iy1,jy) = curry_totalApp v (A := ((h::C)++(n::A))) (tupcat (iy2,tiy) (A:=(h::C)) (iy1,jy) (B:=(n::A)))).
     symmetry. apply recomposition with (i := (iy2,tiy)) (j := (iy1,jy)).
-    simpl in H2. rewrite H2 in H0.
+    simpl in Hy. rewrite Hy in H.
     rewrite Hi,Hj.
-    apply H with (x := (ix2,tupcat tix (ix1,jx) (B := (n::A)))) (y := (iy2,tupcat tiy (iy1,jy) (B := (n::A)))) in H0.
-    injection H0.
-    intros.
-    apply tupcat_injective in H3.
-    injection H3.
-    intros.
-    subst.
+    apply Hinj with (x := (ix2,tupcat tix (ix1,jx) (B := (n::A)))) (y := (iy2,tupcat tiy (iy1,jy) (B := (n::A)))) in H.
+    injection H.
+    intros Hcat Heq.
+    apply tupcat_injective in Hcat.
+    injection Hcat.
+    intros;subst.
     reflexivity.
 Qed.
 
@@ -266,168 +191,198 @@ Proof.
   intros A B.
   induction A.
   + simpl. intros. apply H.
-  + intros. intros. simpl. destruct i.
-      assert (Injective (v i)). {
+  + intros v Hinj i. simpl. destruct i.
+      assert (H:Injective (v i)). {
         unfold Injective.
-        intros. assert ((i,x) = (i,y)).
-        apply H. apply H0. injection H1. trivial.
+        intros x y H. assert ((i,x) = (i,y)).
+        apply Hinj. apply H. injection H0. trivial.
       }
-      apply IHA with (i := t) in H0.
-      apply H0.
+      apply IHA with (i := t) in H.
+      apply H.
 Qed.
 
 
-Lemma lemma1 :
+Lemma injectivity_decomposition :
   forall A B (v : ViewArray (A++B)),
   Injective v -> (forall (i j : Tuple A) (x y : Tuple B), (curry_totalApp (curry_partialApp v i) x) = (curry_totalApp (curry_partialApp v j) y)-> i = j /\ x = y).
 Proof.
-  intros.
+  intros A B v Hinj i j x y H.
   destruct A.
-  - destruct i,j. simpl in H0. apply H in H0. split. reflexivity. apply H0.
+  - destruct i,j. simpl in H. apply Hinj in H. split. reflexivity. apply H.
   - destruct i as [i ti],j as [j tj].
-  simpl in H0.
-  assert (curry_totalApp (curry_partialApp (v i) ti) x = curry_totalApp v (tupcat (i,ti) (A := (h::A)) x)).
-  symmetry. apply recomposition with (i := (i,ti)).
-  assert (curry_totalApp (curry_partialApp (v j) tj) y = curry_totalApp v (tupcat (j,tj) (A := (h::A)) y)).
-  symmetry. apply recomposition with (i := (j,tj)).
-  rewrite H1,H2 in H0.
-  apply H in H0.
-  apply tupcat_injective in H0.
-  injection H0.
-  intros. subst. split;reflexivity.
+    simpl in H.
+    assert (Hx:curry_totalApp (curry_partialApp (v i) ti) x = curry_totalApp v (tupcat (i,ti) (A := (h::A)) x)).
+    symmetry. apply recomposition with (i := (i,ti)).
+    assert (Hy:curry_totalApp (curry_partialApp (v j) tj) y = curry_totalApp v (tupcat (j,tj) (A := (h::A)) y)).
+    symmetry. apply recomposition with (i := (j,tj)).
+    rewrite Hx,Hy in H.
+    apply Hinj in H.
+    apply tupcat_injective in H.
+    injection H.
+    intros; subst. split;reflexivity.
 Qed.
 
-Proposition reverse_preserves_injectivity2 :
+Proposition reverse_preserves_injectivity :
   forall T n, preserveInjectivity reverse (A := (n::T)).
 Proof.
   unfold preserveInjectivity.
-  intros.
-  unfold reverse in H0.
+  intros T n C v Hinj i j x y H.
+  unfold reverse in H.
   destruct x as [x tx],y as [y ty].
-  simpl in H0.
+  simpl in H.
   destruct C.
-  - simpl in *. unfold Injective in H.
-    apply H with (x := ((Id n (n - 1 - to_nat x) reverseProof),tx)) (y := ((Id n (n - 1 - to_nat y) reverseProof),ty)) in H0.
-    inversion H0.
-    apply sub_injective in H2.
-    apply to_nat_injective in H2. subst. destruct i,j. split; reflexivity.
-    destruct n. destruct x. inversion H1. simpl. rewrite Nat.sub_0_r. apply le_S_n. apply BoundedInt.
-    destruct n. destruct y. inversion H1. simpl. rewrite Nat.sub_0_r. apply le_S_n. apply BoundedInt.
+  - simpl in *. unfold Injective in Hinj.
+    apply Hinj with (x := ((Id n (n - 1 - to_nat x) reverseProof),tx)) (y := ((Id n (n - 1 - to_nat y) reverseProof),ty)) in H.
+    inversion H.
+    apply sub_injective in H1.
+    apply to_nat_injective in H1. subst. destruct i,j. split; reflexivity.
+    destruct n. destruct x as [nx Hx]. inversion Hx. simpl. rewrite Nat.sub_0_r. apply le_S_n. apply BoundedInt.
+    destruct n. destruct x as [ny Hy]. inversion Hy. simpl. rewrite Nat.sub_0_r. apply le_S_n. apply BoundedInt.
   - destruct i as [i ti],j as [j tj].
     set (i' := (i,ti)) in *.
     set (x' := ((Id n (n - 1 - to_nat x) reverseProof),tx)) in *.
     set (j' := (j,tj)) in *.
     set (y' := ((Id n (n - 1 - to_nat y) reverseProof),ty)) in *.
-    assert ((curry_totalApp (curry_partialApp v i') x') = (curry_totalApp (curry_partialApp v j') y')-> i' = j' /\ x' = y').
-    apply lemma1. apply H.
+    assert (Heq : (curry_totalApp (curry_partialApp v i') x') = (curry_totalApp (curry_partialApp v j') y')-> i' = j' /\ x' = y').
+    apply injectivity_decomposition. apply Hinj.
     simpl in *.
-    apply H1 in H0. destruct H0.
-    unfold x',y' in H2.
-    inversion H2.
-    apply sub_injective in H4.
-    apply to_nat_injective in H4.
-    unfold i',j' in *. inversion H0. subst. split; reflexivity.
-    destruct n. destruct x. inversion H3. simpl. rewrite Nat.sub_0_r. apply le_S_n. apply BoundedInt.
-    destruct n. destruct y. inversion H3. simpl. rewrite Nat.sub_0_r. apply le_S_n. apply BoundedInt.
+    apply Heq in H. destruct H as [H H'].
+    unfold i',j',x',y' in *.
+    inversion H'.
+    apply sub_injective in H1.
+    apply to_nat_injective in H1.
+    inversion H. subst. split; reflexivity.
+    destruct n. destruct x as [nx Hx]. inversion Hx. simpl. rewrite Nat.sub_0_r. apply le_S_n. apply BoundedInt.
+    destruct n. destruct y as [ny Hy]. inversion Hy. simpl. rewrite Nat.sub_0_r. apply le_S_n. apply BoundedInt.
 Qed.
 
-Proposition select_preserves_injectivity2 :
-  forall T n a b, preserveInjectivity (select a b) (A := (b+n::T)).
+Proposition takeleft_preserves_injectivity :
+  forall T n b, preserveInjectivity (take_left b) (A := (b+n::T)).
 Proof.
   unfold preserveInjectivity.
-  intros.
+  intros T n b C v Hinj i j x y H.
   destruct x as [x tx],y as [y ty].
   destruct C.
-  - unfold select in *.
-    unfold Injective in H.
-    apply H with (x := ((Id (b + n) (a + to_nat x) selectProof),tx)) (y := ((Id (b + n) (a + to_nat y) selectProof),ty)) in H0.
-    inversion H0.
-    apply add_injective in H2.
-    apply to_nat_injective in H2.
+  - unfold take_left in *. simpl in H.
+    unfold Injective in Hinj.
+    apply Hinj with (x := ((Id (b + n) (to_nat x) takeleftProof),tx)) (y := (((Id (b + n) (to_nat y) takeleftProof)),ty)) in H.
+    inversion H.
+    apply to_nat_injective in H1.
     subst. destruct i,j. split;reflexivity.
   - destruct i as [i ti],j as [j tj].
     set (i' := (i,ti)) in *.
-    set (x' := ((Id (b + n) (a + to_nat x) selectProof),tx)) in *.
+    set (x' := ((Id (b + n) (to_nat x) takeleftProof),tx)) in *.
     set (j' := (j,tj)) in *.
-    set (y' := ((Id (b + n) (a + to_nat y) selectProof),ty)) in *.
-    assert ((curry_totalApp (curry_partialApp v i') x') = (curry_totalApp (curry_partialApp v j') y')-> i' = j' /\ x' = y').
-    apply lemma1. apply H.
+    set (y' := ((Id (b + n) (to_nat y) takeleftProof),ty)) in *.
+    assert (Heq:(curry_totalApp (curry_partialApp v i') x') = (curry_totalApp (curry_partialApp v j') y')-> i' = j' /\ x' = y').
+    apply injectivity_decomposition. apply Hinj.
     unfold x',y',i',j' in *.
-    apply H1 in H0.
-    destruct H0.
-    injection H0. intros.
-    inversion H2.
-    apply add_injective in H6.
-    apply to_nat_injective in H6.
+    apply Heq in H.
+    destruct H as [H H'].
+    injection H. intros.
+    inversion H'.
+    apply to_nat_injective in H3.
     subst. split;reflexivity.
 Qed.
 
-Proposition transpose_preserves_injectivity2 :
+Proposition takeright_preserves_injectivity :
+  forall T n a, preserveInjectivity (take_right a) (A := (a+n::T)).
+Proof.
+  unfold preserveInjectivity.
+  intros T n a C v Hinj i j x y H.
+  destruct x as [x tx],y as [y ty].
+  destruct C.
+  - unfold take_right in *. simpl in H.
+    unfold Injective in Hinj.
+    simpl in *.
+    apply Hinj with (x := ((Id (a + n) (a + to_nat x) takerightProof),tx)) (y := (((Id (a + n) (a + to_nat y) takerightProof)),ty)) in H.
+    inversion H.
+    apply add_injective in H1.
+    apply to_nat_injective in H1.
+    subst. destruct i,j. split;reflexivity.
+  - destruct i as [i ti],j as [j tj].
+    set (i' := (i,ti)) in *.
+    set (x' := ((Id (a + n) (a + to_nat x) takerightProof),tx)) in *.
+    set (j' := (j,tj)) in *.
+    set (y' := ((Id (a + n) (a + to_nat y) takerightProof),ty)) in *.
+    assert (Heq:(curry_totalApp (curry_partialApp v i') x') = (curry_totalApp (curry_partialApp v j') y')-> i' = j' /\ x' = y').
+    apply injectivity_decomposition. apply Hinj.
+    unfold x',y',i',j' in *.
+    apply Heq in H.
+    destruct H as [H H'].
+    injection H.
+    inversion H'.
+    apply add_injective in H1.
+    apply to_nat_injective in H1.
+    intros;subst. split;reflexivity.
+Qed.
+
+Proposition transpose_preserves_injectivity :
   forall T m n, preserveInjectivity transpose (A := (m::n::T)).
 Proof.
   unfold preserveInjectivity.
-  intros.
+  intros T m n C v Hinj i j x y H.
   destruct C.
-  - destruct i,j,x as [xi tx], y as [yi ty], tx as [xj tx], ty as [yj ty]. unfold Injective in H.
+  - destruct i,j,x as [xi tx], y as [yi ty], tx as [xj tx], ty as [yj ty]. unfold Injective in Hinj.
     simpl in *.
-    apply H with (x := (xj,(xi,tx))) (y := (yj,(yi,ty))) in H0.
-    injection H0.
-    intros.
-    subst. split;reflexivity.
+    apply Hinj with (x := (xj,(xi,tx))) (y := (yj,(yi,ty))) in H.
+    injection H.
+    intros;subst.
+    split;reflexivity.
   - destruct i as [i ti],j as [j tj].
     destruct x as [xi tx], y as [yi ty], tx as [xj tx], ty as [yj ty].
     set (i' := (i,ti)) in *.
     set (x' := (xj,(xi,tx))) in *.
     set (j' := (j,tj)) in *.
     set (y' := (yj,(yi,ty))) in *.
-    assert ((curry_totalApp (curry_partialApp v i') x') = (curry_totalApp (curry_partialApp v j') y')-> i' = j' /\ x' = y').
-    apply lemma1. apply H.
+    assert (Heq:(curry_totalApp (curry_partialApp v i') x') = (curry_totalApp (curry_partialApp v j') y')-> i' = j' /\ x' = y').
+    apply injectivity_decomposition. apply Hinj.
     unfold x',y',i',j' in *.
-    apply H1 in H0.
-    destruct H0.
-    injection H0. injection H2. intros. subst.
+    apply Heq in H.
+    destruct H as [H H'].
+    injection H. injection H'. intros; subst.
     split;reflexivity.
 Qed.
 
-Proposition group_preserves_injectivity2 :
+Proposition group_preserves_injectivity :
   forall T m n, preserveInjectivity (group m) (A := (m*n::T)).
 Proof.
   unfold preserveInjectivity.
-  intros.
+  intros T m n C v Hinj i j x y H.
   destruct C.
-  - destruct i,j,x as [xi tx], y as [yi ty], tx as [xj tx], ty as [yj ty]. unfold Injective in H.
-    unfold group in H0.
+  - destruct i,j,x as [xi tx], y as [yi ty], tx as [xj tx], ty as [yj ty]. unfold Injective in Hinj.
+    unfold group in H.
     simpl in *.
-    apply H with
+    apply Hinj with
       (x := (Id (m * n) (to_nat xj + m * to_nat xi) groupProof,tx))
       (y := (Id (m * n) (to_nat yj + m * to_nat yi) groupProof,ty))
-     in H0.
-    inversion H0.
-    apply projection_injective in H2.
-    injection H2.
-    intros.
-    apply to_nat_injective in H1,H4.
+     in H.
+    inversion H.
+    apply projection_injective in H1.
+    injection H1.
+    intros Hx Hy.
+    apply to_nat_injective in Hx,Hy.
     subst. split;reflexivity.
     apply BoundedInt.
     apply BoundedInt.
   - destruct i as [i ti],j as [j tj],x as [xi tx], y as [yi ty], tx as [xj tx], ty as [yj ty].
-  set (i' := (i,ti)) in *.
-  set (x' := (Id (m * n) (to_nat xj + m * to_nat xi) groupProof,tx)) in *.
-  set (j' := (j,tj)) in *.
-  set (y' := (Id (m * n) (to_nat yj + m * to_nat yi) groupProof,ty)) in *.
-  assert ((curry_totalApp (curry_partialApp v i') x') = (curry_totalApp (curry_partialApp v j') y')-> i' = j' /\ x' = y').
-  apply lemma1. apply H.
-  apply H1 in H0.
-  unfold i',j',x',y' in *.
-  destruct H0.
-  injection H0.
-  inversion H2.
-  apply projection_injective in H4.
-  inversion H4.
-  apply to_nat_injective in H6,H7.
-  intros. subst. split;reflexivity.
-  apply BoundedInt.
-  apply BoundedInt.
+    set (i' := (i,ti)) in *.
+    set (x' := (Id (m * n) (to_nat xj + m * to_nat xi) groupProof,tx)) in *.
+    set (j' := (j,tj)) in *.
+    set (y' := (Id (m * n) (to_nat yj + m * to_nat yi) groupProof,ty)) in *.
+    assert (Heq:(curry_totalApp (curry_partialApp v i') x') = (curry_totalApp (curry_partialApp v j') y')-> i' = j' /\ x' = y').
+    apply injectivity_decomposition. apply Hinj.
+    apply Heq in H.
+    unfold i',j',x',y' in *.
+    destruct H as [H H'].
+    injection H.
+    inversion H'.
+    apply projection_injective in H1.
+    inversion H1.
+    apply to_nat_injective in H3,H4.
+    intros; subst. split;reflexivity.
+    apply BoundedInt.
+    apply BoundedInt.
 Qed.
 
 
@@ -435,46 +390,43 @@ Proposition map_preserves_injectivity :
   forall A B (n : nat) (f : ViewArray A -> ViewArray B), preserveInjectivity f -> preserveInjectivity (map f (n := n)).
 Proof.
   unfold preserveInjectivity.
-  intros.
+  intros A B n f Hf C v Hinj i j x y H.
   destruct C.
   - destruct i,j,x as [xi tx], y as [yi ty].
     simpl in *.
-    unfold map in H1.
-    assert (curry_totalApp (f (curry_partialApp v (A := (n::[])) (xi,I))) tx = curry_totalApp (f (curry_partialApp v (A := (n::[])) (yi,I))) ty ->
+    unfold map in H.
+    assert (Heq:curry_totalApp (f (curry_partialApp v (A := (n::[])) (xi,I))) tx = curry_totalApp (f (curry_partialApp v (A := (n::[])) (yi,I))) ty ->
       (xi,I) = (yi,I) /\ tx = ty).
-    apply H with (i := (xi,I)) (j := (yi,I)).
-    apply H0.
-    simpl in H2.
-    apply H2 in H1.
-    destruct H1.
-    injection H1.
-    intros.
-    subst.
+    apply Hf with (i := (xi,I)) (j := (yi,I)).
+    apply Hinj.
+    simpl in Heq.
+    apply Heq in H.
+    destruct H as [H H'].
+    injection H.
+    intros;subst.
     split;reflexivity.
   - destruct i as [i ti],j as [j tj],x as [xi tx], y as [yi ty].
     unfold map in *.
     set (v' := reorder v (C := (h::C))).
-    assert (curry_partialApp v (A := (h::C)) (i,ti) xi = curry_partialApp (reorder v (C := (h::C))) (A := (n::h::C)) (xi,(i,ti))).
+    assert (Hx:curry_partialApp v (A := (h::C)) (i,ti) xi = curry_partialApp (reorder v (C := (h::C))) (A := (n::h::C)) (xi,(i,ti))).
     apply reorder_is_correct.
-    assert (curry_partialApp v (A := (h::C)) (j,tj) yi = curry_partialApp (reorder v (C := (h::C))) (A := (n::h::C)) (yi,(j,tj))).
+    assert (Hy:curry_partialApp v (A := (h::C)) (j,tj) yi = curry_partialApp (reorder v (C := (h::C))) (A := (n::h::C)) (yi,(j,tj))).
     apply reorder_is_correct.
     simpl in *.
-    rewrite H2 in H1.
-    rewrite H3 in H1.
+    rewrite Hx,Hy in H.
     set (i' := (xi,(i,ti))) in *.
     set (x' := tx) in *.
     set (j' := (yi,(j,tj))) in *.
     set (y' := ty) in *.
-    assert (curry_totalApp (f (curry_partialApp (reorder v (C := (h::C))) (A := (n::h::C)) i')) x' = curry_totalApp (f (curry_partialApp (reorder v (C := (h::C))) (A := (n::h::C)) j')) y' ->
+    assert (Heq:curry_totalApp (f (curry_partialApp (reorder v (C := (h::C))) (A := (n::h::C)) i')) x' = curry_totalApp (f (curry_partialApp (reorder v (C := (h::C))) (A := (n::h::C)) j')) y' ->
     i' = j' /\ x' = y').
-    apply H.
+    apply Hf.
     apply reorder_keeps_injectivity.
-    apply H0.
+    apply Hinj.
     unfold i',j',x',y' in *.
-    apply H4 in H1.
-    destruct H1.
-    injection H1.
-    intros.
-    subst.
+    apply Heq in H.
+    destruct H as [H H'].
+    injection H.
+    intros;subst.
     split;reflexivity.
 Qed.
